Flow/Analysis/Utils.lean
@@ -1,0 +1,30 @@
+import Mathlib.Tactic.Lemma
+
+namespace Utils
+
+lemma sum_map_update_le {B : Type} [DecidableEq B]
+      (l : List B) (f : B -> Nat) (n : B) (nv : Nat) (hle : f n ≤ nv) :
+    (l.map f).sum ≤ (l.map (fun x => if x = n then nv else f x)).sum := by
+  induction l with
+  | nil => grind
+  | cons h t ih =>
+    simp only [List.map_cons, List.sum_cons]
+    by_cases h' : h = n
+    case pos => simpa [h'] using Nat.add_le_add hle ih
+    case neg => simpa [h'] using ih
+
+lemma sum_map_update_lt {B : Type} [DecidableEq B]
+      (l : List B) (f : B -> Nat) (n : B) (nv : Nat)
+      (hin : n ∈ l) (hlt : f n < nv) :
+    (l.map f).sum < (l.map (fun x => if x = n then nv else f x)).sum := by
+  induction l with
+  | nil => cases hin
+  | cons h t ih =>
+    by_cases hc : h = n
+    case pos =>
+      simp only [hc, List.map_cons, List.sum_cons, ↓reduceIte]
+      refine Nat.add_lt_add_of_lt_of_le hlt ?_
+      exact sum_map_update_le t f n nv (by grind)
+    case neg => grind
+
+end Utils
